consistency almost proven

coq/SystemFCProp.v
@@ -44,36 +44,209 @@ Proof.
   exists t0. trivial.
 Qed.
 
-Lemma homogeneity_sym : forall U V,
-  types_homogeneous U V ->
-  types_homogeneous V U.
-Proof with auto.
-  intros; induction H; try (apply homogeneity_refl); constructor...
+(* Lemma coercion_unique : forall c Gamma U1 U2 V1 V2, *)
+(*   Gamma |- c ; U1 ~ U2 -> *)
+(*   Gamma |- c ; V1 ~ V2 -> *)
+(*   U1 = V1 /\ U2 = V2. *)
+(* Proof. *)
+(*   intros; generalize dependent V1; generalize dependent V2; *)
+(*   coercion_cases (induction H) Case; inversion H0; subst. *)
+(*   Case "C_Var". *)
+(*     rewrite H1 in H4. inversion H4. split; trivial. *)
+(*   Case "C_Refl". *)
+(*     split; trivial. *)
+(*   Case "C_Sym". *)
+    
+Inductive types_consistent : ty -> ty -> Prop :=
+  | TC_Arrow : forall U1 U2 V1 V2,
+    types_consistent (TArrow U1 U2) (TArrow V1 V2)
+  | TC_Univ : forall U V,
+    types_consistent (TUniv U) (TUniv V)
+  | TC_Coerce : forall U1 U2 U3 V1 V2 V3,
+    types_consistent (TCoerce U1 U2 U3) (TCoerce V1 V2 V3).
+
+Fixpoint type_size (T:ty) : nat :=
+  match T with
+  | TVar _ => 1
+  | TArrow T1 T2 => 1 + type_size T1 + type_size T2
+  | TUniv T1     => 1 + type_size T1
+  | TCoerce T1 T2 T3 => 1 + type_size T1 + type_size T2 + type_size T3
+  end.
+
+Fixpoint coercion_size (c:cn) : nat :=
+  match c with
+  | CVar Y            => 1
+  | CRefl T           => 1 + type_size T
+  | CSym c            => 1 + coercion_size c
+  | CTrans c1 c2      => 1 + coercion_size c1 + coercion_size c2
+  | CArrow c1 c2      => 1 + coercion_size c1 + coercion_size c2
+  | CTCoerce c1 c2 c3 => 1 + coercion_size c1 + coercion_size c2 +
+                         coercion_size c3
+  | CNth n c          => 1 + coercion_size c
+  | CTAbs c           => 1 + coercion_size c
+  | CTApp c T         => 1 + coercion_size c + type_size T
+  end.
+
+Lemma ty_size_gt_0 : forall T,
+  type_size T > 0.
+Proof.
+  intros. induction T; simpl; omega.
 Qed.
 
-Lemma homogeneity_trans : forall U V W,
-  types_homogeneous U V ->
-  types_homogeneous V W ->
-  types_homogeneous U W.
-Proof with auto.
-  intros; generalize dependent U; generalize dependent W;
-  induction V; intros; inversion H; inversion H0; subst;
-  try (apply homogeneity_refl); constructor...
+Lemma cn_size_gt_0 : forall c,
+  coercion_size c > 0.
+Proof.
+  intros. induction c; simpl; omega.
 Qed.
 
-Lemma coercion_homogeneity : forall Gamma c U V,
-  Gamma |- c ; U ~ V ->
-  types_homogeneous U V.
+Lemma cn_size_1 : forall c,
+  coercion_size c = 1 ->
+  exists X, c = CVar X.
 Proof with auto.
-  intros; coercion_cases (induction H) Case; trivial;
-  try (apply homogeneity_refl); try (eapply homogeneity_trans; eassumption);
-  try (apply homogeneity_sym; assumption);
-  try (apply subst_preserves_homogeneity);
-  try (inversion IHwell_formed_coercion; assumption);
-  try (inversion IHwell_formed_coercion1);
-  try (inversion IHwell_formed_coercion2);
-  try constructor...
+  intros. induction c;
+  inversion H;
+  try (assert (type_size t > 0) by apply ty_size_gt_0; omega);
+  try (assert (coercion_size c > 0) by apply cn_size_gt_0; omega);
+  try (assert (coercion_size c1 > 0) by apply cn_size_gt_0; omega);
+  exists n...
 Qed.
+
+Lemma admissibility : forall c S T,
+  empty |- c ; S ~ T ->
+  (forall U1 U2 V1 V2,
+     S = TArrow U1 U2 /\ T = TArrow V1 V2 ->
+     exists c1 c2,
+       empty |- c1 ; U1 ~ V1 /\
+       empty |- c2 ; U2 ~ V2 /\
+       coercion_size c1 < coercion_size c /\
+       coercion_size c2 < coercion_size c) /\
+  (forall U V,
+     S = TUniv U /\ T = TUniv V ->
+     exists c1,
+       ext_tvar empty |- c1 ; U ~ V /\
+       coercion_size c1 < coercion_size c) /\
+  (forall U1 U2 U3 V1 V2 V3,
+     S = TCoerce U1 U2 U3 /\ T = TCoerce V1 V2 V3 ->
+     exists c1 c2 c3,
+       empty |- c1 ; U1 ~ V1 /\
+       empty |- c2 ; U2 ~ V2 /\
+       empty |- c3 ; U3 ~ V3 /\
+       coercion_size c1 < coercion_size c /\
+       coercion_size c2 < coercion_size c /\
+       coercion_size c3 < coercion_size c).
+Proof.
+  intros. remember empty as Gamma.
+  coercion_cases (induction H) Case; subst; split; intros; try split; intros.
+  Case "C_Var".
+    inversion H0. inversion H0. inversion H0.
+  Case "C_Refl".
+    SCase "Arrow".
+      inversion H1; subst.
+      exists (CRefl U1). exists (CRefl U2).
+      inversion H3; subst. inversion H0.
+      split. constructor; trivial.
+      split. constructor; trivial.
+      split; simpl; omega.
+    SCase "Univ".
+      inversion H1; subst.
+      exists (CRefl V).
+      inversion H3; subst. inversion H0.
+      split. constructor. constructor. trivial. trivial.
+      simpl. omega.
+    SCase "Coerce".
+      inversion H1; subst.
+      exists (CRefl U1). exists (CRefl U2). exists (CRefl U3).
+      inversion H3; subst. inversion H0; subst.
+      split. constructor; trivial.
+      split. constructor; trivial.
+      split. constructor; trivial.
+      split; simpl; omega.
+Admitted.
+
+Lemma consistency_sym : forall U V,
+  types_consistent U V ->
+  types_consistent V U.
+Proof.
+  intros. inversion H; constructor.
+Qed.
+
+Lemma consistency_trans : forall U V W,
+  types_consistent U V ->
+  types_consistent V W ->
+  types_consistent U W.
+Proof.
+  intros. inversion H; inversion H0; subst; try constructor;
+  try inversion H0.
+Qed.
+
+Lemma subst_preserves_consistency : forall U V n (T:ty),
+  types_consistent U V ->
+  types_consistent ([n := T] U) ([n := T] V).
+Proof.
+  intros. induction H; simpl; constructor.
+Qed.
+
+Lemma coercion_consistency : forall c U V,
+  empty |- c ; U ~ V ->
+  types_consistent U V.
+Proof with eauto.
+  intros. remember (coercion_size c) as n.
+  generalize dependent c; generalize dependent U; generalize dependent V; 
+  induction n using strong_induction; intros.
+  coercion_cases (inversion H0) Case; subst; try constructor;
+  try (apply admissibility in H1; inversion H1; clear H1; clear H3;
+       pose proof (H2 _ _ _ _ (conj eq_refl eq_refl));
+       destruct H1; destruct H1; destruct H1; destruct H3; destruct H4);
+  try (apply admissibility in H1; destruct H1; clear H1;
+       destruct H2; clear H1;
+       pose proof (H2 _ _ _ _ _ _ (conj eq_refl eq_refl));
+       destruct H1; destruct H1; destruct H1; destruct H1; destruct H3;
+       destruct H4; destruct H5; destruct H6).
+  Case "C_Var".
+    inversion H2.
+  Case "C_Refl".
+    admit.
+  Case "C_Sym".
+    apply consistency_sym. apply H with (coercion_size c0) c0;
+    simpl. omega; trivial. trivial. trivial.
+  Case "C_Trans".
+    apply consistency_trans with V0.
+    apply H with (coercion_size c1) c1; try (simpl; omega); trivial. 
+    apply H with (coercion_size c2) c2; try (simpl; omega); trivial.
+  Case "C_ALeft".
+    apply H with (coercion_size x) x; try (simpl; omega); trivial.
+  Case "C_ARight".
+    apply H with (coercion_size x0) x0; try (simpl; omega); trivial.
+  Case "C_CLeft11".
+    apply H with (coercion_size x) x; try (simpl; omega); trivial.
+  Case "C_CLeft12".
+    apply H with (coercion_size x0) x0; try (simpl; omega); trivial.
+  Case "C_CRight".
+    apply H with (coercion_size x1) x1; try (simpl; omega); trivial.
+  Case "C_Inst".
+    apply subst_preserves_consistency.
+    apply admissibility in H1; destruct H1; destruct H3; clear H1; clear H4.
+    pose proof (H3 _ _ (conj eq_refl eq_refl)). destruct H1.
+    destruct H1.
+    apply H with (coercion_size x) x; try (simpl; omega); trivial.
+    
+
+
+Lemma canonical_coercion_abs : forall c T U1 U2,
+  (empty |- c ; T ~ TArrow U1 U2 \/
+   empty |- c ; TArrow U1 U2 ~ T) ->
+  exists V1 V2, T = TArrow V1 V2.
+Proof with eauto.
+  intros; remember empty as Gamma; remember (TArrow U1 U2) as V.
+  generalize dependent U1; generalize dependent U2.
+  coercion_cases (induction H) Case; intros...
+  Case "C_Var".
+    subst; inversion H0.
+  Case "C_Sym".
+    
+ 
+    pose (IHwell_formed_coercion eq_refl U2 U1).
+
 
 (* ###################################################################### *)
 (** * Progress *)
