coq/Evaluation.v
@@ -1,11 +1,11 @@
 Require Export Substitution.
-Require Export Shifting.
+Require Export Typing.
 
 Module EVALUATION.
 Import SYSTEMFC.
 Import SHIFTING.
 Import SUBSTITUTION.
-
+Import TYPING.
 
 (* ################################### *)
 (** *** Reduction *)
@@ -14,16 +14,11 @@ Import SUBSTITUTION.
 Reserved Notation "t1 '==>' t2" (at level 40).
 
 Inductive step : tm -> tm -> Prop :=
-  | E_AppAbs : forall T t12 v2,
-         value v2 ->
-         (tapp (tabs T t12) v2) ==> [0:=v2]t12
-  | E_App1 : forall t1 t1' t2,
+  | E_AppAbs : forall T t12 t2,
+         (tapp (tabs T t12) t2) ==> [0:=t2]t12
+  | E_App : forall t1 t1' t2,
          t1 ==> t1' ->
          tapp t1 t2 ==> tapp t1' t2
-  | E_App2 : forall v1 t2 t2',
-         value v1 ->
-         t2 ==> t2' -> 
-         tapp v1 t2 ==> tapp v1 t2'
   | E_TApp : forall t1 t1' T2,
          t1 ==> t1' ->
          ttapp t1 T2 ==> ttapp t1' T2
@@ -40,17 +35,19 @@ Inductive step : tm -> tm -> Prop :=
   | E_CTrans : forall c1 c2 v,
          uncoerced_value v ->
          tcoerce (tcoerce v c1) c2 ==> tcoerce v (CTrans c1 c2)
-  | E_PushApp : forall v1 v2 c,
-         uncoerced_value v1 ->
-         value v2 ->
-         tapp (tcoerce v1 c) v2 ==>
-              tcoerce (tapp v1 (tcoerce v2 (CSym (CNth 1 c)))) (CNth 2 c)
-  | E_PushTApp : forall v T c,
-         uncoerced_value v        ->
+  | E_PushApp : forall v1 t2 c U1 U2,
+         uncoerced_value v1           ->
+         empty |- v1 \in TArrow U1 U2 ->
+         tapp (tcoerce v1 c) t2 ==>
+              tcoerce (tapp v1 (tcoerce t2 (CSym (CNth 1 c)))) (CNth 2 c)
+  | E_PushTApp : forall v T c U,
+         uncoerced_value v      ->
+         empty |- v \in TUniv U ->
          ttapp (tcoerce v c) T ==>
               tcoerce (ttapp v T) (CTApp c T)
-  | E_PushCApp : forall v c c0,
-         uncoerced_value v ->
+  | E_PushCApp : forall v c c0 U1 U2 U,
+         uncoerced_value v              ->
+         empty |- v \in TCoerce U1 U2 U ->
          tcapp (tcoerce v c0) c ==>
                tcoerce (tcapp v (CTrans (CTrans (CNth 1 (CNth 1 c0)) c)
                                         (CSym (CNth 2 (CNth 1 c0)))))
@@ -60,8 +57,8 @@ where "t1 '==>' t2" := (step t1 t2).
 
 Tactic Notation "step_cases" tactic(first) ident(c) :=
   first;
-  [ Case_aux c "E_AppAbs"   | Case_aux c "E_App1" 
-  | Case_aux c "E_App2"     | Case_aux c "E_TApp" 
+  [ Case_aux c "E_AppAbs"   | Case_aux c "E_App" 
+  | Case_aux c "E_TApp" 
   | Case_aux c "E_TAppTAbs" | Case_aux c "E_CApp"
   | Case_aux c "E_CAppCAbs" | Case_aux c "E_Coerce"
   | Case_aux c "E_CTrans"   | Case_aux c "E_PushApp"
